Saving a lot of work, basically all proofs but Disclose and ManComp are done

src/Attestation_Session.v
@@ -4,10 +4,11 @@ Require Import JSON Stringifiable.
 Import ListNotations.
 
 Record Attestation_Session := 
-  mkAtt_Sesplit_evt {
+  mkAtt_Sess {
   Session_Plc     : Plc ;
   Plc_Mapping     : MapC Plc UUID;
   PubKey_Mapping  : MapC Plc PublicKey;
+  ats_context     : GlobalContext
 }.
 
 Inductive DispatcherErrors : Type :=
@@ -32,23 +33,22 @@ Record Session_Config := {
 }.
 
 Open Scope string_scope.
-Global Instance Jsonifiable_Attestation_Session `{Jsonifiable (MapC Plc UUID), Jsonifiable (MapC Plc PublicKey)}: Jsonifiable Attestation_Session.
+Global Instance Jsonifiable_Attestation_Session `{Jsonifiable (MapC Plc UUID), Jsonifiable (MapC Plc PublicKey), Jsonifiable GlobalContext}: Jsonifiable Attestation_Session.
 eapply Build_Jsonifiable with 
   (to_JSON := (fun v => 
                 JSON_Object [
                   ("Session_Plc", JSON_String (to_string (Session_Plc v)));
                   ("Plc_Mapping", to_JSON (Plc_Mapping v));
-                  ("PubKey_Mapping", to_JSON (PubKey_Mapping v))])) 
+                  ("PubKey_Mapping", to_JSON (PubKey_Mapping v));
+                  ("Session_Context", to_JSON (ats_context v))])) 
   (from_JSON := (fun j =>
-    match (JSON_get_string "Session_Plc" j), (JSON_get_Object "Plc_Mapping" j), (JSON_get_Object "PubKey_Mapping" j) with
-    | resultC plc, resultC plc_map, resultC pub_map =>
-        match (from_string plc), (from_JSON plc_map), (from_JSON pub_map) with
-        | resultC plc', resultC plc_map', resultC pub_map' =>
-            resultC {| Session_Plc := plc'; Plc_Mapping := plc_map'; PubKey_Mapping := pub_map' |}
-        | _, _, _ => errC "Error in parsing Attestation_Session"
+    match (JSON_get_string "Session_Plc" j), (JSON_get_Object "Plc_Mapping" j), (JSON_get_Object "PubKey_Mapping" j), (JSON_get_Object "Session_Context" j) with
+    | resultC plc, resultC plc_map, resultC pub_map, resultC sc =>
+        match (from_string plc), (from_JSON plc_map), (from_JSON pub_map), (from_JSON sc) with
+        | resultC plc', resultC plc_map', resultC pub_map', resultC sc =>
+            resultC {| Session_Plc := plc'; Plc_Mapping := plc_map'; PubKey_Mapping := pub_map'; ats_context := sc |}
+        | _, _, _, _ => errC "Error in parsing Attestation_Session"
         end
-    | _, _, _ => errC "Error in parsing Attestation_Session"
-    end)).
-simpl in *; intuition.
-repeat rewrite canonical_jsonification; destruct a; eauto.
+    | _, _, _, _ => errC "Error in parsing Attestation_Session"
+    end)); solve_json.
 Defined.
