src/Cvm_Monad.v
@@ -309,14 +309,14 @@ Definition check_cvm_policy (t:Term) (pTo:Plc) (et:EvidenceT) : CVM unit :=
 Definition do_remote (sc : Session_Config) (pTo: Plc) (e : Evidence) (t:Term) 
     : ResultT Evidence DispatcherErrors := 
   (* There is assuredly a better way to do it than this *)
-  let '(mkAtt_Sesplit_evt my_plc plc_map pk_map) := (session_config_decompiler sc) in
+  let '(mkAtt_Sess my_plc plc_map pk_map G) := (session_config_decompiler sc) in
   (* We need  to update the Att Session to tell the next plc how
   they should be tagging their stuff (basically who they are
   in the protocol) *)
-  let new_att_sesplit_evt := (mkAtt_Sesplit_evt pTo plc_map pk_map) in
+  let new_att_sess := (mkAtt_Sess pTo plc_map pk_map G) in
   match (map_get plc_map pTo) with 
   | Some uuid => 
-      let remote_req := (mkPRReq new_att_sesplit_evt my_plc e t) in
+      let remote_req := (mkPRReq new_att_sess my_plc e t) in
       let js_req := to_JSON remote_req in
       let resp_res := make_JSON_Network_Request uuid js_req in
       match resp_res with
@@ -379,7 +379,7 @@ Definition start_par_thread (t: Term) (e:Evidence) : CVM nat :=
 Definition do_wait_par_thread (loc:Loc) (p:Plc) (e:Evidence) (t: Term) : CVM Evidence :=
   match (parallel_vm_thread loc p e t) with
   | resultC e' => err_ret e'
-  | errC s => err_failm (dispatch_error (Runtime s))
+  | errC s => err_failm s
   end.
 
 Definition wait_par_thread (loc:Loc) (e:Evidence) (t: Term) : CVM Evidence :=
