src/AM_Json_Interfaces.v
@@ -1,57 +1,8 @@
 Require Import List.
 Import ListNotations.
 Require Import BS Term_Defs Attestation_Session Interface String IO_Stubs Manifest_Admits ErrorStMonad_Coq AM_Monad Session_Config_Compiler.
-Require Import ErrorStringConstants Impl_appraisal Cvm_Run AM_Manager.
+Require Import ErrorStringConstants Cvm_Run AM_Manager.
 Import ErrNotation.
-
-Definition am_check_auth_tok (t:Term) (fromPl:Plc) (authTok:ReqAuthTok) 
-    : AM AppResultC :=
-  match authTok with
-  | evc auth_ev auth_et => 
-    appres <-
-    (match (requester_bound t fromPl authTok) with
-     | false => am_failm (am_error errStr_requester_bound)
-     | true => gen_appraise_AM auth_et auth_ev
-     end) ;;
-    err_ret appres
-  end.
-(* 
-Definition am_serve_auth_tok_req (t:Term) (fromPl : Plc) 
-                                 (authTok:ReqAuthTok) (init_ev:RawEv) (ac : AM_Config) (al:AM_Library) : AM RawEv :=
-  let test_print := print_auth_tok authTok in
-  v <- am_check_auth_tok t fromPl authTok ;;
-  match ((appraise_auth_tok v)) with
-  | true =>
-
-    config_AM_if_lib_supported (absMan ac) al ;; 
-  
-    (*
-    check_disclosure_policy t myPlc init_et ;;
-    (* TODO: decide how to get initial EvidenceT type here for server AMs...  *)
-    *)
-    
-    ret (run_cvm_rawEv t init_ev ac)
-    (*
-    | false => am_failm (am_error errStr_disclosePolicy)
-    end *)
-      
-  | false => am_failm (am_error errStr_app_auth_tok)
-  end. *)
-
-Definition do_appraisal_session (conf : AM_Manager_Config) (appreq:ProtocolAppraiseRequest) (nonceVal:BS)
-    : ResultT ProtocolAppraiseResponse string :=
-  let '(mkPAReq att_sesplit_evt t p et ev) := appreq in
-  let expected_et := eval t p et in 
-  let app_am := gen_appraise_AM expected_et ev in 
-  let init_noncemap := [(O, nonceVal)] in
-  let init_nonceid := (S O) in
-  let sess_config := (session_config_compiler conf att_sess) in
-  let my_amst := (mkAM_St init_noncemap init_nonceid sess_config) in
-  match run_am_app_comp_init app_am my_amst with
-  | errC e => errC e
-  | resultC appres =>
-      resultC (mkPAResp true appres)
-  end.
 
 Definition handle_AM_request_JSON (conf : AM_Manager_Config) (js : JSON) (nonceVal:BS) : JSON :=
   match (JSON_get_string STR_ACTION js) with
@@ -62,9 +13,9 @@ Definition handle_AM_request_JSON (conf : AM_Manager_Config) (js : JSON) (nonceV
       match (from_JSON js) with
       | errC msg => ErrorResponseJSON msg
       | resultC r =>
-        let '(mkPRReq att_sesplit_evt cop_term from_plc ev) := r in
+        let '(mkPRReq att_sess from_plc ev cop_term) := r in
         let sc := (session_config_compiler conf att_sess) in
-        let cvm_resp := (run_cvm_rawEv cop_term ev sc) in
+        let cvm_resp := (run_cvm_init_ev sc ev cop_term) in
         match cvm_resp with
         | errC e => ErrorResponseJSON e
         | resultC res_ev => to_JSON (mkPRResp true res_ev)
@@ -76,36 +27,5 @@ Definition handle_AM_request_JSON (conf : AM_Manager_Config) (js : JSON) (nonceV
       (* TODO: Fill this in when negotiation is implemented *)
       ErrorResponseJSON errStr_negotiation_not_implemented
     )
-    else if (eqb req_type STR_APPRAISE)
-    then (
-      match (from_JSON js) with
-      | errC msg => ErrorResponseJSON msg
-      | resultC appreq =>
-        let app_resp := (do_appraisal_session conf appreq nonceVal) in 
-        match app_resp with
-        | errC e => ErrorResponseJSON e
-        | resultC app_resp => to_JSON app_resp
-        end
-      end
-    )
     else ErrorResponseJSON "Invalid request type"
-  end.
-
-Definition make_AM_Protocol_Run_request_JSON (att_sesplit_evt : Attestation_Session)
-    (t:Term) (targ_uuid : UUID) (tok:ReqAuthTok) (ev:RawEv) (from_plc : Plc)
-    : ResultT RawEv string :=
-  let req := (mkPRReq att_sesplit_evt t from_plc ev) in
-  let js_req := to_JSON req in
-  let resp_res := make_JSON_Network_Request targ_uuid js_req in
-  match resp_res with
-  | resultC js_resp =>
-      match from_JSON js_resp with
-      | resultC prresp =>
-        let '(mkPRResp success ev) := prresp in
-        if success 
-        then resultC ev 
-        else errC errStr_remote_am_failure
-      | errC msg => errC msg
-      end
-  | errC msg => errC msg
   end.
