src/Cvm_Axioms.v
@@ -1,0 +1,39 @@
+Require Import IO_Stubs ResultT Cvm_Monad Attestation_Session Cvm_Impl.
+
+Axiom parallel_vm_thread_res_axiom : forall i t e e' p,
+  parallel_vm_thread i p e t = resultC e' ->
+  forall st sc,
+    st = {| st_ev := e; st_trace := nil; st_evid := i; st_config := sc |} ->
+    session_plc sc = p ->
+    exists st' u,
+      build_cvm t st = (resultC u, st') /\ st_ev st' = e'.
+
+Axiom parallel_vm_thread_err_axiom : forall i t e p err,
+  parallel_vm_thread i p e t = errC err ->
+  forall st sc,
+    st = {| st_ev := e; st_trace := nil; st_evid := i; st_config := sc |} ->
+    session_plc sc = p ->
+    exists st',
+      build_cvm t st = (errC err, st').
+
+Axiom do_remote_res_axiom : forall sc p e t e',
+  do_remote sc p e t = resultC e' ->
+  forall st sc' i,
+    (* NOTE: This is maybe a bit stronger than we want!
+    we really need to be looking at the NEW session config that was
+    created via the passed session *)
+    st = {| st_ev := e; st_trace := nil; st_evid := i; st_config := sc' |} ->
+    exists st' u,
+      build_cvm t st = (resultC u, st') /\ st_ev st' = e' /\
+      session_plc sc' = p /\
+      session_context sc' = session_context sc.
+
+Axiom do_remote_err_axiom : forall sc p e t s,
+  do_remote sc p e t = errC s ->
+  forall st sc' i,
+    (* NOTE: This is maybe a bit stronger than we want!
+    we really need to be looking at the NEW session config that was
+    created via the passed session *)
+    st = {| st_ev := e; st_trace := nil; st_evid := i; st_config := sc' |} ->
+    exists st',
+      build_cvm t st = (errC (dispatch_error s), st').
