src/Extraction_Cvm_Cake.v
@@ -7,7 +7,7 @@ Require Import Term_Defs Term_Defs_Core Cvm_Run IO_Stubs AM_Monad Cvm_Monad.
 
 Require Import Manifest_Generator Session_Config_Compiler.
 
-Require Import AM_Helpers Server_AM Client_AM.
+Require Import AM_Helpers Server_AM.
 
 Require Import Manifest_Generator_Union Manifest_JSON Flexible_Mechanisms.
 
@@ -32,10 +32,10 @@ Extract Inlined Constant Nat.eqb => "(op=)".
 Separate Extraction 
     full_flexible_mechanisms
     run_cvm session_config_compiler 
-		handle_AM_request end_to_end_mangen_final
-    run_demo_client_AM concrete_Jsonifiable_Manifest
+		handle_AM_request end_to_end_mangen
+    concrete_Jsonifiable_Manifest
     concrete_Jsonifiable_ASP_Compat_MapT
     concrete_Jsonifiable_Attestation_Session
     concrete_Jsonifiable_Term
     concrete_Jsonifiable_EvidenceT
-    Jsonifiable_EvidenceT_Plc_list Jsonifiable_Term_Plc_list.
+    Jsonifiable_Term_Plc_list.
