src/Flexible_Mechanisms.v
@@ -6,51 +6,51 @@ Import ListNotations.
 Definition certificate_style : Term :=
   att P1 (
     lseq 
-      (asp (ASPC ALL (EXTD 1) (asp_paramsC attest_id [] P1 sys_targ)))
+      (asp (ASPC ALL (asp_paramsC attest_id [] P1 sys_targ)))
       (att P2 (
         lseq 
-          (asp (ASPC ALL (EXTD 1) (asp_paramsC appraise_id [] P2 sys_targ)))
-          (asp (ASPC ALL (EXTD 1) (asp_paramsC certificate_id [] P2 sys_targ)))
+          (asp (ASPC ALL (asp_paramsC appraise_id [] P2 sys_targ)))
+          (asp (ASPC ALL (asp_paramsC certificate_id [] P2 sys_targ)))
       ))
   ).
 
 Definition background_check : Term :=
   lseq
-    (att P1 (asp (ASPC ALL (EXTD 1) (asp_paramsC attest_id [] P1 sys_targ))))
-    (att P2 (asp (ASPC ALL (EXTD 1) (asp_paramsC appraise_id [] P2 sys_targ)))).
+    (att P1 (asp (ASPC ALL (asp_paramsC attest_id [] P1 sys_targ))))
+    (att P2 (asp (ASPC ALL (asp_paramsC appraise_id [] P2 sys_targ)))).
 
 Definition parallel_mutual_1 : Term :=
   att P1 (
     lseq 
-      (asp (ASPC ALL (EXTD 1) (asp_paramsC attest_id [] P1 sys_targ)))
-      (att P2 (asp (ASPC ALL (EXTD 1) (asp_paramsC appraise_id [] P2 sys_targ))))
+      (asp (ASPC ALL (asp_paramsC attest_id [] P1 sys_targ)))
+      (att P2 (asp (ASPC ALL (asp_paramsC appraise_id [] P2 sys_targ))))
   ).
 
 Definition parallel_mutual_2 : Term :=
   att P0 (
     lseq 
-      (asp (ASPC ALL (EXTD 1) (asp_paramsC attest_id [] P0 sys_targ)))
-      (att P2 (asp (ASPC ALL (EXTD 1) (asp_paramsC appraise_id [] P2 sys_targ))))
+      (asp (ASPC ALL (asp_paramsC attest_id [] P0 sys_targ)))
+      (att P2 (asp (ASPC ALL (asp_paramsC appraise_id [] P2 sys_targ))))
   ).
 
 Definition layered_background_check : Term :=
   att P1
     (bpar (ALL, ALL)
       (lseq
-        (att P1 (asp (ASPC ALL (EXTD 1) (asp_paramsC attest_id [] P1 sys_targ))))
+        (att P1 (asp (ASPC ALL (asp_paramsC attest_id [] P1 sys_targ))))
         (lseq 
-          (asp (ASPC ALL (EXTD 1) (asp_paramsC attest_id [] P3 att_targ)))
-          (asp (ASPC ALL (EXTD 1) (asp_paramsC attest_id [] P4 att_targ)))
+          (asp (ASPC ALL (asp_paramsC attest_id [] P3 att_targ)))
+          (asp (ASPC ALL (asp_paramsC attest_id [] P4 att_targ)))
         )
       )
       (bpar (ALL, ALL)
-        (att P3 (asp (ASPC ALL (EXTD 1) (asp_paramsC attest_id [] P3 sys_targ))))
+        (att P3 (asp (ASPC ALL (asp_paramsC attest_id [] P3 sys_targ))))
         (lseq
-          (att P4 (asp (ASPC ALL (EXTD 1) (asp_paramsC attest_id [] P4 sys_targ))))
+          (att P4 (asp (ASPC ALL (asp_paramsC attest_id [] P4 sys_targ))))
           (att P2 (
             (lseq
-              (asp (ASPC ALL (EXTD 1) (asp_paramsC appraise_id [] P2 it_targ)))
-              (asp (ASPC ALL (EXTD 1) sig_params))
+              (asp (ASPC ALL (asp_paramsC appraise_id [] P2 it_targ)))
+              (asp (ASPC ALL sig_params))
             )
           )
           )
@@ -61,7 +61,7 @@ Definition layered_background_check : Term :=
 Definition filehash_auth_phrase : Term := 
   att P1 
     (lseq 
-      (asp (ASPC ALL (EXTD 1) (asp_paramsC hashfile_id [] P1 hashfile_targ)))
+      (asp (ASPC ALL (asp_paramsC hashfile_id [] P1 hashfile_targ)))
       (asp SIG) 
     ).
 
@@ -75,7 +75,8 @@ Definition flexible_mechanisms_map :=
    ("filehash", filehash_auth_phrase)].
 
 Definition add_EvidenceT_flexible_mechanisms := 
-  Maps.map_map (fun t => (t, eval t P0 (nonce_evt 0))) flexible_mechanisms_map.
+  fun G =>
+  Maps.map_map (fun t => (t, eval G P0 (nonce_evt 0) t)) flexible_mechanisms_map.
 
 Definition full_flexible_mechanisms :=
   add_EvidenceT_flexible_mechanisms.
