src/Helpers_CvmSemantics.v
@@ -4,7 +4,7 @@ Helper lemmas for proofs about the CVM semantics.
 Author:  Adam Petz, ampetz@ku.edu
 *)
 
-Require Import Cvm_Monad Cvm_Impl Term_Defs Auto Attestation_Session StructTactics AutoApp.
+Require Import Cvm_Monad Cvm_Impl Term_Defs Defs Attestation_Session StructTactics Cvm_Axioms Term.
 Require Import Coq.Program.Tactics.
 
 Import ListNotations.
@@ -13,8 +13,7 @@ Lemma sc_immut_peel_n_rawev : forall n r st res st',
   peel_n_rawev n r st = (res, st') ->
   st_config st = st_config st'.
 Proof.
-  induction n; simpl in *; intuition; cvm_monad_unfold;
-  ff.
+  induction n; simpl in *; intuition; cvm_monad_unfold; ff.
 Qed.
 
 Lemma peel_n_rawev_deterministic : forall n r st1 st2 res1 res2 st1' st2',
@@ -58,6 +57,36 @@ Proof.
       intuition; clear H1;
       try congruence; repeat find_injection
   end.
+Qed.
+
+Lemma peel_n_rawev_result_spec : forall n ls ls1 ls2 st st',
+  (peel_n_rawev n ls) st = (resultC (ls1, ls2), st') ->
+  ls = ls1 ++ ls2 /\ length ls1 = n.
+Proof.
+  induction n; ffa using cvm_monad_unfold; ffl.
+Qed.
+
+Lemma peel_n_none_spec : forall n ls e st st',
+  (peel_n_rawev n ls) st = (errC e, st') ->
+  length ls < n.
+Proof.
+  induction n; ffa using cvm_monad_unfold; ffl.
+Qed.
+
+Lemma peel_n_rawev_state_immut : forall n r st res st',
+  peel_n_rawev n r st = (res, st') ->
+  st = st'.
+Proof.
+  induction n; ffa using cvm_monad_unfold.
+Qed.
+
+Lemma split_evidence_state_immut : forall r et1 et2 res st st',
+  split_evidence r et1 et2 st = (res, st') ->
+  st = st'.
+Proof.
+  intros.
+  unfold split_evidence in *; cvm_monad_unfold; ff;
+  repeat find_eapply_lem_hyp peel_n_rawev_state_immut; ff.
 Qed.
 
 Lemma sc_immut_invoke_APPR : forall et st r st',
@@ -138,6 +167,34 @@ Proof.
     repeat find_rewrite; eauto.
 Qed.
 
+Theorem invoke_APPR_deterministic_Evidence : forall et st1 st2 r1 r2 st1' st2',
+  st_config st1 = st_config st2 ->
+  st_ev st1 = st_ev st2 ->
+  invoke_APPR et st1 = (r1, st1') ->
+  invoke_APPR et st2 = (r2, st2') ->
+  r1 = r2 /\ st_ev st1' = st_ev st2'.
+Proof.
+  induction et; ffa using cvm_monad_unfold;
+  match goal with
+  | H1 : split_evidence _ _ _ _ = _,
+    H2 : split_evidence _ _ _ _ = _ |- _ =>
+    let H' := fresh in
+    eapply split_evidence_determinisitic in H1 as H';
+    try eapply H2; ff; 
+    eapply split_evidence_state_immut in H1;
+    eapply split_evidence_state_immut in H2;
+    simpl in *; ff
+  end;
+  match goal with
+  | H1 : invoke_APPR ?e _ = _,
+    H2 : invoke_APPR ?e _ = _,
+    IH : context[invoke_APPR ?e _ = _ -> _] |- _ =>
+    eapply IH in H1; try eapply H2; ff
+  end;
+  try (repeat find_eapply_lem_hyp sc_immut_invoke_APPR; ff; fail).
+  eapply IHet1 in Heqp3; try eapply Heqp0; ff.
+Qed.
+
 (* Theorem EvidenceT_deterministic_output_on_results : forall t e tr1 tr2 i1 i2 ac st1 st2,
   build_cvm t {| st_ev := e; st_trace := tr1; st_evid := i1; st_config := ac |} = (resultC tt, st1) ->
   build_cvm t {| st_ev := e; st_trace := tr2; st_evid := i2; st_config := ac |} = (resultC tt, st2) ->
@@ -200,25 +257,134 @@ Lemma cvm_deterministic :  forall t st1 st2 r1 r2 st1' st2',
     (st_config st1' = st_config st2')
   ).
 Proof.
-  induction t; intros;
-  try (simpl in *; cvm_monad_unfold; ff;
-  repeat match goal with
+  induction t; simpl in *; cvm_monad_unfold; ff;
+  try (repeat match goal with
   | u : unit |- _ => destruct u
   | H1 : build_cvm ?t _ = _,
     H2 : build_cvm ?t _ = _,
     IH : context[build_cvm ?t _ = _ -> _] |- _ =>
       eapply IH in H1; try (eapply H2);
       clear IH H2; try (intuition; congruence)
-  end; intuition; symmetry; ff).
-  - simpl in *; cvm_monad_unfold;
-    destruct a; simpl in *;
-    try (repeat find_injection;
-      simpl in *; intuition; fail);
-    try destruct s; simpl in *;
-    repeat find_rewrite; try ff;
-    find_eapply_lem_hyp invoke_APPR_deterministic; eauto;
-    intuition; eauto; try congruence;
-    destruct u; eauto.
+  end; fail);
+  find_eapply_lem_hyp invoke_APPR_deterministic; ff;
+  try congruence;
+  match goal with
+  | u : unit |- _ => destruct u
+  end; eauto.
+Qed.
+
+Lemma asp_events_errs_deterministic : forall G t p e i1 i2 e1 e2,
+  asp_events G p e t i1 = resultC e1 ->
+  asp_events G p e t i2 = errC e2 ->
+  False.
+Proof.
+  destruct t; ff; try (destruct e; simpl in *; congruence);
+  generalizeEverythingElse e;
+  induction e; ffa using result_monad_unfold.
+Qed.
+
+Lemma events_fix_errs_deterministic : forall G t p e i1 i2 e1 e2,
+  events_fix G p e t i1 = resultC e1 ->
+  events_fix G p e t i2 = errC e2 ->
+  False.
+Proof.
+  induction t; ffa using result_monad_unfold.
+  destruct a; simpl in *;
+  try (destruct e; simpl in *; congruence).
+  generalizeEverythingElse e.
+  induction e; ffa using result_monad_unfold.
+Qed.
+
+Lemma events_fix_only_one_error : forall G t p e i1 i2 e1 e2,
+  events_fix G p e t i1 = errC e1 ->
+  events_fix G p e t i2 = errC e2 ->
+  e1 = e2.
+Proof.
+  induction t; ffa using result_monad_unfold;
+  try match goal with
+  | H1 : events_fix _ _ _ ?t _ = resultC _,
+    H2 : events_fix _ _ _ ?t _ = errC _ |- _ =>
+    eapply events_fix_errs_deterministic in H1; try eapply H2; ff; fail
+  end.
+  destruct a; simpl in *;
+  try (destruct e; simpl in *; congruence).
+  generalizeEverythingElse e;
+  induction e; ffa using result_monad_unfold;
+  try match goal with
+  | H1 : asp_events _ _ ?e _ _ = resultC _,
+    H2 : asp_events _ _ ?e _ _ = errC _ |- _ =>
+    eapply asp_events_errs_deterministic in H1; try eapply H2; ff; fail
+  end.
+Qed.
+
+Theorem cvm_deterministic_Evidence : forall t st1 st2 r1 r2 st1' st2',
+  st_config st1 = st_config st2 ->
+  st_ev st1 = st_ev st2 ->
+  build_cvm t st1 = (r1, st1') ->
+  build_cvm t st2 = (r2, st2') ->
+  r1 = r2 /\ st_ev st1' = st_ev st2'.
+Proof.
+  induction t; simpl in *; cvm_monad_unfold.
+  - ff;
+    match goal with
+    | H1 : invoke_APPR _ _ = _,
+      H2 : invoke_APPR _ _ = _ |- _ =>
+      eapply invoke_APPR_deterministic_Evidence in H1;
+      try eapply H2; ff
+    end.
+  - ff; (* NOTE: Why dont we need the remote axiom here!? *)
+    match goal with
+    | H1 : events_fix _ _ _ ?t _ = _,
+      H2 : events_fix _ _ _ ?t _ = _ |- _ =>
+      try (eapply events_fix_only_one_error in H1; try eapply H2; ff; fail);
+      try (eapply events_fix_errs_deterministic in H1; try eapply H2; ff; fail)
+    end.
+  - ff; repeat match goal with
+    | u : unit |- _ => destruct u
+    | H1 : build_cvm ?t _ = _,
+      H2 : build_cvm ?t _ = _,
+      IH : context[build_cvm ?t _ = _ -> _] |- _ =>
+        eapply sc_immut_better in H1 as ?;
+        eapply sc_immut_better in H2 as ?;
+        simpl in *; ff;
+        eapply IH in H1; try (eapply H2);
+        clear IH H2; try (intuition; congruence)
+    end.
+  - ff; repeat match goal with
+    | u : unit |- _ => destruct u
+    | H1 : build_cvm ?t _ = _,
+      H2 : build_cvm ?t _ = _,
+      IH : context[build_cvm ?t _ = _ -> _] |- _ =>
+        eapply sc_immut_better in H1 as ?;
+        eapply sc_immut_better in H2 as ?;
+        simpl in *; ff;
+        eapply IH in H1; try (eapply H2);
+        clear IH H2; try (intuition; congruence)
+    end.
+  - ff; simpl in *; 
+    repeat match goal with
+    | u : unit |- _ => destruct u
+    | H : parallel_vm_thread _ _ _ _ = resultC _ |- _ => 
+      eapply parallel_vm_thread_res_axiom in H;
+      try reflexivity; break_exists
+    | H : parallel_vm_thread _ _ _ _ = errC _ |- _ => 
+      eapply parallel_vm_thread_err_axiom in H;
+      try reflexivity; break_exists
+    | H1 : build_cvm ?t _ = _,
+      H2 : build_cvm ?t _ = _,
+      IH : context[build_cvm ?t _ = _ -> _] |- _ =>
+        eapply sc_immut_better in H1 as ?;
+        eapply sc_immut_better in H2 as ?;
+        simpl in *; ff;
+        eapply IH in H1; try (eapply H2);
+        clear IH H2; try (intuition; congruence)
+    end;
+    match goal with
+    | H1 : events_fix _ _ _ ?t _ = _,
+      H2 : events_fix _ _ _ ?t _ = _ |- _ =>
+      try (eapply events_fix_only_one_error in H1; try eapply H2; ff; fail);
+      try (eapply events_fix_errs_deterministic in H1; try eapply H2; ff; fail)
+    end.
 Qed.
 
 (* Lemma stating the following:  If all starting parameters to the cvm_st are the same, except 
@@ -231,7 +397,7 @@ Lemma st_trace_irrel : forall t e e' e'' x x' y y' i i' i'' ac ac' ac'' res,
     (e' = e'' /\ i' = i'' /\ ac' = ac'').
 Proof.
   intros; find_eapply_lem_hyp cvm_deterministic; 
-  try eapply H; simpl in *; intuition; eauto.
+  try eapply H; ff.
 Qed.
 
 Ltac do_st_trace :=
